theories/case_studies/multiuser_kvs/kvs_spec_read_safe.v
@@ -1,4 +1,3 @@
-From griotte Require Import kvs_spec_read_general.
 From iris.proofmode Require Import proofmode.
 From griotte Require Import proofmode map_simpl register_tactics.
 From griotte Require Import logrel rules.
@@ -117,7 +116,7 @@ Section KVS_spec_read_safe.
 
     (* Either the map key is already allocated, or it is not *)
     iDestruct "Hinterp_nkey" as "[ (%w & >Hney & #Hinterp_nkey) | >Hnkey ]".
-    - iApply KVS_read_spec_in_general; last iFrame "∗#"; eauto.
+    - iApply KVS_read_spec_in; last iFrame "∗#"; eauto.
       iNext.
       iIntros "(Hna & HPC & Hgcp & Hcra & Hca0 & [%actual [Hca1 %Hactual]] & Hct1 & Hct2 & Hctp & Hcnull
                 & Ha & HLUKVS & Hnkey)".
