theories/switcher/switcher_helpers.v
@@ -42,6 +42,7 @@ Section switcher_helper.
   Lemma open_world_interp_cframe
     (W : WORLD) (C : CmptName) (b_stk e_stk a_stk a_stk4 : Addr)
     (wret wcgp0 wcs2 wcs3 : Word) (ccrel : caller_callee_relation)
+    (scgp scra scs0 scs1 : option bool)
     :
     (b_stk <= a_stk)%a ->
     (a_stk ^+ 3 < e_stk)%a ->
@@ -56,7 +57,11 @@ Section switcher_helper.
         b_stk := b_stk;
         a_stk := a_stk;
         e_stk := e_stk;
-        ccrel := ccrel
+        ccrel := ccrel;
+        shadow_cgp := scgp;
+        shadow_cra := scra;
+        shadow_cs0 := scs0;
+        shadow_cs1 := scs1
       |}
     ∗ world_interp W C
       -∗
@@ -199,7 +204,8 @@ Section switcher_helper.
 
     Lemma open_world_interp_cframe_gen
     (W0 Wcur : WORLD) (C : CmptName) (b_stk csp_b csp_e a_stk4 : Addr) (l : list Addr)
-    (wret wcgp wcs0 wcs1 : Word) (ccrel : caller_callee_relation) :
+    (wret wcgp wcs0 wcs1 : Word) (ccrel : caller_callee_relation)
+    (scgp scra scs0 scs1 : option bool) :
       let Wfixed := close_list (l ++ finz.seq_between csp_b csp_e) Wcur in
       let a_stk := (csp_b ^+ -4)%a in
 
@@ -221,8 +227,12 @@ Section switcher_helper.
           b_stk := b_stk;
           a_stk := a_stk;
           e_stk := csp_e;
-          ccrel := ccrel
-        |}
+          ccrel := ccrel;
+          shadow_cgp := scgp;
+          shadow_cra := scra;
+          shadow_cs0 := scs0;
+          shadow_cs1 := scs1
+      |}
         -∗
         close_list_resources_gen C Wcur (l ++ finz.seq_between csp_b csp_e) l false -∗
         £ 1
